trans: Prove atomicity WIP
Signed-off-by: Kyeongmin Cho <kyeongmin.cho@kaist.ac.kr>

src/examples/transaction.v
@@ -1,6 +1,7 @@
 Require Import PArith.
 Require Import ZArith.
 Require Import List.
+Require RelationClasses.
 Import ListNotations.
 
 Require Import sflib.
@@ -27,7 +28,7 @@ From Memento Require Import DR.
   r2 := pcas(loc_1002, val_0, val_42, mid_2)
   r0 := pcas(loc_1000, val_1, val_0, mid_3)
 *)
-Definition prog := [
+Definition transaction := [
   (stmt_pcas
     (Pos.of_nat 0)
     (expr_reg (Pos.of_nat 1000))
@@ -58,11 +59,16 @@ Definition prog := [
   )
 ].
 
-Lemma prog_rw:
+Definition consistent_state (mem: Mem.t) :=
+  mem (PLoc.int 1000) = Val.int 0 ->
+  (mem (PLoc.int 1001) = Val.int 0 /\ mem (PLoc.int 1002) = Val.int 0)
+  \/ (mem (PLoc.int 1001) = Val.int 41 /\ mem (PLoc.int 1002) = Val.int 42).
+
+Lemma transaction_rw:
   forall envt,
-    exists labs, EnvType.rw_judge envt labs prog.
+    exists labs, EnvType.rw_judge envt labs transaction.
 Proof.
-  i. unfold prog. esplits.
+  i. unfold transaction. esplits.
   econs 10; cycle 4.
   { instantiate (2 := [_]). instantiate (1 := [_; _; _]). ss. }
   all: cycle 1.
@@ -106,13 +112,59 @@ Proof.
   inv H0. inv H.
 Qed.
 
-Lemma prog_DR:
+(* TODO: durability 증명할 때 필요. terminated 됐을 때 0 41 42가 있어야 함 *)
+Lemma transaction_DR:
   forall env envt,
     TypeSystem.judge env envt ->
-  DR env prog.
+  DR env transaction.
 Proof.
-  i. hexploit prog_rw. i. des.
+  i. hexploit transaction_rw. i. des.
   eapply DR_RW; eauto.
   admit. (* DR trivial lemma *)
 Qed.
 
+Lemma transaction_atomic_step:
+  forall p envt s c ts mmts tr mach mach_term,
+    p = prog_intro envt (IdMap.add (Pos.of_nat 1) transaction (IdMap.empty _)) ->
+    IdMap.find (Pos.of_nat 1) mach.(Machine.tmap) = Some (Thread.mk s c ts mmts) ->
+    suffix_of s transaction ->
+    consistent_state mach.(Machine.mem) ->
+    Machine.step p tr mach mach_term ->
+  consistent_state mach_term.(Machine.mem).
+Proof.
+  admit.
+Qed.
+
+Lemma transaction_atomic_rtc_step:
+  forall p envt s c ts mmts tr mach mach_term,
+    p = prog_intro envt (IdMap.add (Pos.of_nat 1) transaction (IdMap.empty _)) ->
+    IdMap.find (Pos.of_nat 1) mach.(Machine.tmap) = Some (Thread.mk s c ts mmts) ->
+    suffix_of s transaction ->
+    consistent_state mach.(Machine.mem) ->
+    Machine.rtc p tr mach mach_term ->
+  consistent_state mach_term.(Machine.mem).
+Proof.
+  i. revert envt s c ts mmts H2 H1 H0 H. induction H3; i; [ ss |]. subst.
+  hexploit Machine.step_suffix_of_prog; eauto.
+  { admit. }
+  intro SUFFIX.
+
+  hexploit transaction_atomic_step; eauto. i.
+
+  specialize (SUFFIX (Pos.of_nat 1)).
+  inv SUFFIX. destruct (Machine.tmap mach0); ss. subst. destruct b.
+  eapply IHrtc; eauto.
+Qed.
+
+Theorem transaction_atomic:
+  forall p envt tr mach_term,
+    p = prog_intro envt (IdMap.add (Pos.of_nat 1) transaction (IdMap.empty _)) ->
+    Machine.rtc p tr (Machine.init p) mach_term ->
+  consistent_state mach_term.(Machine.mem).
+Proof.
+  i.
+  assert (INIT_CONST: consistent_state (Machine.init p).(Machine.mem)).
+  { left. ss. }
+  subst.
+  eapply transaction_atomic_rtc_step; eauto; [econs | refl].
+Qed.
